trace experiments: finished lemma about get state returning the last set state

src/core/DY.Core.Trace.Experiments.fst
@@ -9,73 +9,33 @@ open DY.Core.Label.Type
 
 #set-options "--fuel 1 --ifuel 1"
 
-
 let rec trace_concat tr1 tr2 =
   match tr2 with
   | Nil -> tr1
   | Snoc init2 ev2 ->
       Snoc (trace_concat tr1 init2) ev2
       
-#push-options "--fuel 2"
-let trace_concat_singleton_lemma tr1 ev :
-  Lemma (trace_concat tr1 (Snoc Nil ev) = Snoc tr1 ev)
-  [SMTPat (trace_concat tr1 (Snoc Nil ev))]
-= ()
-#pop-options
 
-let rec trace_concat_event_exists_lemma tr1 tr2 :
-  Lemma (forall ev. event_exists tr1 ev \/ event_exists tr2 ev ==> event_exists (trace_concat tr1 tr2) ev) =
-  match tr2 with
-  | Nil -> ()
-  | Snoc init _ -> trace_concat_event_exists_lemma tr1 init
+val trace_concat_grows:
+  tr1:trace -> tr2:trace ->
+  Lemma (tr1 <$ trace_concat tr1 tr2)
+  [SMTPat (trace_concat tr1 tr2)]
+let rec trace_concat_grows tr1 tr2 =
+    reveal_opaque (`%grows) (grows);
+    norm_spec [zeta; delta_only [`%prefix]] (prefix);
+    match tr2 with
+    | Nil -> ()
+    | Snoc init ev -> 
+           trace_concat_grows tr1 init
 
-val exists_set_state_entry_for:
-  principal -> state_id -> trace -> prop
-let exists_set_state_entry_for p sid tr = 
-  exists (ts:nat{ts < DY.Core.Trace.Type.length tr}). 
-      match get_event_at tr ts with
-      | SetState p' sid' _ -> p' = p && sid' = sid
-      | _ -> False
-  
 val no_set_state_entry_for:
   principal -> state_id -> trace -> prop
 let no_set_state_entry_for p sid tr = 
-//   ~ ( exists_set_state_entry_for p sid tr)
   forall (ts:timestamp{ts < DY.Core.Trace.Type.length tr}).
     match get_event_at tr ts with
     | SetState p' sid' _ -> p' <> p \/ sid' <> sid
     | _ -> True
 
-#push-options "--fuel 2"
-val no_set_state_entry_for_snoc :
-  p:principal -> sid:state_id -> tr:trace -> ev:trace_event ->
-  Lemma
-    (requires 
-       no_set_state_entry_for p sid tr /\
-       (match ev with
-        | SetState p' sid' _ -> p' <> p \/ sid' <> sid
-        | _ -> True
-       )
-    )
-    (ensures no_set_state_entry_for p sid (Snoc tr ev))
-let no_set_state_entry_for_snoc p sid tr ev = ()
-#pop-options
-
-// TODO: hier weiter machen
-#push-options "--fuel 2"
-val no_set_state_entry_for_concat:
- p:principal -> sid:state_id -> tr1:trace -> tr2:trace -> 
- Lemma 
-   (requires no_set_state_entry_for p sid tr1 /\ no_set_state_entry_for p sid tr2)
-   (ensures no_set_state_entry_for p sid (trace_concat tr1 tr2))
-let rec no_set_state_entry_for_concat p sid tr1 tr2 = 
-  match tr2 with
-  | Nil -> admit()
-  | Snoc init (SetState p' sid' v) ->  
-         assert(event_at tr2 (DY.Core.Trace.Type.length tr2 -1) (SetState p' sid' v));
-         assume(no_set_state_entry_for p sid init);
-         no_set_state_entry_for_concat p sid tr1 init
-  | Snoc init _ -> admit()
 
 #push-options "--fuel 2"
 let _ = 
@@ -85,35 +45,25 @@ let _ =
   let tr = Nil in
   assert(no_set_state_entry_for p sid tr);
   let tr' = Snoc Nil (SetState p sid b) in
-//  assert(DY.Core.Trace.Type.length tr' = 1);
   assert(get_event_at tr' 0 = SetState p sid b);
-  assert(exists_set_state_entry_for p sid tr');
+  assert(~(no_set_state_entry_for p sid tr'));
   assert(no_set_state_entry_for "b" sid tr')
 #pop-options
 
-val suffix_after_event_aux:
-  ev:trace_event -> tr:trace{event_exists tr ev} -> trace -> trace
-let rec suffix_after_event_aux the_ev tr accum =
-  match tr with
-  | Snoc init ev ->
-      if ev <> the_ev 
-        then suffix_after_event_aux the_ev init (Snoc accum ev)
-        else accum
+val no_set_state_entry_for_prefix:
+  p:principal -> sid:state_id -> tr1:trace -> tr2:trace ->
+  Lemma 
+    (requires no_set_state_entry_for p sid tr2 /\ tr1 <$ tr2)
+    (ensures no_set_state_entry_for p sid tr1)
+    [SMTPat (no_set_state_entry_for p sid tr2); SMTPat (tr1 <$ tr2)]
+let no_set_state_entry_for_prefix p sid tr1 tr2 = 
+  introduce forall (ts:timestamp{ts < DY.Core.Trace.Type.length tr1}). get_event_at tr1 ts = get_event_at tr2 ts
+  with begin
+    let ev1 = get_event_at tr1 ts in
+    event_at_grows tr1 tr2 ts ev1
+    end
 
-val suffix_after_event:
-  ev:trace_event -> tr:trace{event_exists tr ev} -> trace
-let suffix_after_event ev tr = suffix_after_event_aux ev tr Nil
 
-#push-options "--fuel 2"
-let _ =
-  let ev1 = MsgSent (Literal FStar.Seq.Base.empty) in
-  let ev2 = Corrupt "p" {the_id = 1} in
-  let tr = Snoc (Snoc Nil ev1) ev2 in
-  assert(suffix_after_event ev2 tr = Nil);
-  assert(suffix_after_event ev1 tr = Snoc Nil ev2);
-  let tr' = Snoc (Snoc (Snoc Nil ev1) ev1) ev2 in  
-  assert(suffix_after_event ev1 tr' = Snoc Nil ev2)
-#pop-options
 
 val get_state_aux_state_was_set :
   p:principal -> sid:state_id -> tr:trace ->
@@ -134,12 +84,34 @@ let rec get_state_aux_state_was_set p sid tr =
        then begin
          let ev = (SetState p' sid' v) in
          assert(event_at tr (DY.Core.Trace.Type.length tr - 1) ev)
-//         assert(event_exists tr (SetState p' sid' v))
        end
        else get_state_aux_state_was_set p sid init
   | Snoc init _ -> get_state_aux_state_was_set p sid init
 
-#push-options "--fuel 4"
+
+val suffix_after_event:
+  ev:trace_event -> tr:trace{event_exists tr ev} -> trace
+let rec suffix_after_event the_ev tr =
+  match tr with
+  | Snoc init ev ->
+      if ev <> the_ev 
+        then Snoc (suffix_after_event the_ev init) ev
+        else Nil
+
+
+#push-options "--fuel 2"
+let _ =
+  let ev1 = MsgSent (Literal FStar.Seq.Base.empty) in
+  let ev2 = Corrupt "p" {the_id = 1} in
+  let tr = Snoc (Snoc Nil ev1) ev2 in
+  assert(suffix_after_event ev2 tr = Nil);
+  assert(suffix_after_event ev1 tr = Snoc Nil ev2);
+  let tr' = Snoc (Snoc (Snoc Nil ev1) ev1) ev2 in  
+  assert(suffix_after_event ev1 tr' = Snoc Nil ev2)
+#pop-options
+
+
+#push-options "--fuel 2"
 val get_state_aux_returns_last_set_state : 
   p:principal -> sid:state_id -> tr:trace ->
   Lemma
@@ -151,6 +123,7 @@ val get_state_aux_returns_last_set_state :
          (suffix_after_event (SetState p sid v) tr)
      )
    )
+   [SMTPat (get_state_aux p sid tr)]
 let rec get_state_aux_returns_last_set_state p sid tr =
   match get_state_aux p sid tr with
   | None -> ()
@@ -158,21 +131,9 @@ let rec get_state_aux_returns_last_set_state p sid tr =
       match tr with
       | Nil -> ()
       | Snoc init (SetState p' sid' v') ->
-          if p' = p && sid' = sid
-            then ()
-            else begin 
-              get_state_aux_returns_last_set_state p sid init
-              ; assert(no_set_state_entry_for p sid 
-                  (suffix_after_event (SetState p sid v) init)
-                  )
-              ; assert(forall tr1 tr2. no_set_state_entry_for p sid tr1 /\ no_set_state_entry_for p sid tr2 ==> no_set_state_entry_for p sid (trace_concat tr1 tr2))
-              ; assume(suffix_after_event (SetState p sid v) tr 
-                  = Snoc (suffix_after_event (SetState p sid v) init)
-                      (SetState p' sid' v')
-                  )
-              ; trace_concat_singleton_lemma (suffix_after_event (SetState p sid v) init) (SetState p' sid' v')      
-              ; assert(no_set_state_entry_for p sid (Snoc Nil (SetState p' sid' v')))
-//              ; admit()
-            end
-      | Snoc init _ -> admit()
-  end
+            get_state_aux_returns_last_set_state p sid init
+      | Snoc init ev ->
+             assert(event_exists init (SetState p sid v));
+             get_state_aux_returns_last_set_state p sid init
+    end
+#pop-options
